ironfleet/src/Dafny/Distributed/Protocol/RSL/FailureProof/Failover2/FailureHelpers.i.dfy
@@ -26,7 +26,47 @@ function {:opaque} TBEpoch2() : Timestamp
 // TODO: move these to a different file
 function {:opaque} EpochQD(nextActionIndex:int) : Timestamp
 {
-  0
+  if nextActionIndex == 8 then
+    StepToTimeDelta(RslStep(7))
+  else if nextActionIndex == 9 then
+    StepToTimeDelta(RslStep(7)) + StepToTimeDelta(RslStep(8))
+  else if nextActionIndex == 0 then
+    StepToTimeDelta(RslStep(7)) + StepToTimeDelta(RslStep(8)) + StepToTimeDelta(RslStep(9))
+  else if nextActionIndex == 1 then
+    StepToTimeDelta(RslStep(7)) + StepToTimeDelta(RslStep(8)) + StepToTimeDelta(RslStep(9)) +
+    Timeout() +
+    StepToTimeDelta(RslStep(0))
+  else if nextActionIndex == 2 then
+    StepToTimeDelta(RslStep(7)) + StepToTimeDelta(RslStep(8)) + StepToTimeDelta(RslStep(9)) +
+    Timeout() +
+    StepToTimeDelta(RslStep(0)) + StepToTimeDelta(RslStep(1))
+  else if nextActionIndex == 3 then
+    StepToTimeDelta(RslStep(7)) + StepToTimeDelta(RslStep(8)) + StepToTimeDelta(RslStep(9)) +
+    Timeout() +
+    StepToTimeDelta(RslStep(0)) + StepToTimeDelta(RslStep(1)) + StepToTimeDelta(RslStep(2))
+  else if nextActionIndex == 4 then
+    StepToTimeDelta(RslStep(7)) + StepToTimeDelta(RslStep(8)) + StepToTimeDelta(RslStep(9)) +
+    Timeout() +
+    StepToTimeDelta(RslStep(0)) + StepToTimeDelta(RslStep(1)) + StepToTimeDelta(RslStep(2)) +
+    StepToTimeDelta(RslStep(3))
+  else if nextActionIndex == 5 then
+    StepToTimeDelta(RslStep(7)) + StepToTimeDelta(RslStep(8)) + StepToTimeDelta(RslStep(9)) +
+    Timeout() +
+    StepToTimeDelta(RslStep(0)) + StepToTimeDelta(RslStep(1)) + StepToTimeDelta(RslStep(2)) +
+    StepToTimeDelta(RslStep(3)) + StepToTimeDelta(RslStep(4))
+  else if nextActionIndex == 6 then
+    StepToTimeDelta(RslStep(7)) + StepToTimeDelta(RslStep(8)) + StepToTimeDelta(RslStep(9)) +
+    Timeout() +
+    StepToTimeDelta(RslStep(0)) + StepToTimeDelta(RslStep(1)) + StepToTimeDelta(RslStep(2)) +
+    StepToTimeDelta(RslStep(3)) + StepToTimeDelta(RslStep(4)) + StepToTimeDelta(RslStep(5))
+  else if nextActionIndex == 7 then
+    StepToTimeDelta(RslStep(7)) + StepToTimeDelta(RslStep(8)) + StepToTimeDelta(RslStep(9)) +
+    Timeout() +
+    StepToTimeDelta(RslStep(0)) + StepToTimeDelta(RslStep(1)) + StepToTimeDelta(RslStep(2)) +
+    StepToTimeDelta(RslStep(3)) + StepToTimeDelta(RslStep(4)) + StepToTimeDelta(RslStep(5)) +
+    StepToTimeDelta(RslStep(6))
+  else
+    0
 }
 
 function {:opaque} HeartbeatQD(nextActionIndex:int) : Timestamp
@@ -36,7 +76,7 @@ function {:opaque} HeartbeatQD(nextActionIndex:int) : Timestamp
 
 function {:opaque} HBPeriodEnd() : Timestamp
 {
-  TBEpoch2() // + HBPeriod()
+  TBEpoch2() + EpochQD(7) + StepToTimeDelta(RslStep(7)) + HBPeriod
 }
 
 function {:opaque} TBFirstSuspectingHB() : Timestamp
@@ -50,11 +90,6 @@ function {:opaque} TBBecomeSuspector() : Timestamp
 }
 
 function {:opaque} TBJustBeforeNewView() : Timestamp
-{
-  0 // TODO
-}
-
-function {:opaque} TBFirstNewViewHB() : Timestamp
 {
   0 // TODO
 }
